additional/gcd_clean.dfy
@@ -1,0 +1,23 @@
+// Try to prove here that `exists q1: int :: q1 * gcd == a` and same for b.
+
+
+method greatest_common_divisor(a: nat, b: nat) returns (result: nat)
+{
+    var x := a;
+    var y := b;
+    
+ 
+    while (y != 0 && x != 0)
+    {
+        if x > y {
+            x := x % y;
+        } else {
+            y := y % x;
+        }
+    }
+    if x != 0 {
+        result := x;
+    } else {
+        result := y;
+    }
+}
