additional/gcd_done.dfy
@@ -1,0 +1,72 @@
+function gcd(a: int, b: int) : (result : int)
+    requires a >= 0
+    requires b >= 0
+{
+    if (b == 0) then a else
+    if (a == 0) then b else
+    if (a > b) then gcd(a % b, b) else
+    if (b > a) then gcd(a, b % a) else a
+}
+
+lemma gcd_correct(a: int, b: int)
+    requires a >= 0
+    requires b >= 0
+
+    ensures (exists q1:int :: (q1 * gcd(a,b) == a))
+    ensures (exists q2:int :: (q2 * gcd(a,b) == b))
+{
+    if (b == 0) 
+    {
+        assert 1 * gcd(a,b) == a;
+        assert 0 * gcd(a,b) == b;
+    }
+    else if (a == 0)
+    {
+        assert 1 * gcd(a,b) == b;
+        assert 0 * gcd(a,b) == a;
+    }
+    else if (a > b)
+    {
+        gcd_correct(a % b, b);
+        var q1 :| q1 * gcd(a % b,b) == a % b;
+        var q2 :| q2 * gcd(a % b,b) == b;
+        assert (q1+q2 * (a / b)) * gcd(a,b) == a;
+    }
+    else
+    {
+        gcd_correct(a, b % a);
+        var q1 :| q1 * gcd(a,b % a) == b % a;
+        var q2 :| q2 * gcd(a,b % a) == a;
+        assert (q1+q2 * (b / a)) * gcd(a,b) == b;
+    }
+}
+
+method greatest_common_divisor(a: nat, b: nat) returns (result: nat)
+    requires a != 0 || b != 0
+    ensures result == gcd(a, b)
+    ensures (exists q1: int :: (q1 * result == a))
+    ensures (exists q2: int :: (q2 * result == b))
+{
+    var x := a;
+    var y := b;
+    
+ 
+    while (y != 0 && x != 0)
+        decreases x+y
+        invariant x >= 0
+        invariant y >= 0
+        invariant gcd(x,y) == gcd(a,b)
+    {
+        if x > y {
+            x := x % y;
+        } else {
+            y := y % x;
+        }
+    }
+    if x != 0 {
+        result := x;
+    } else {
+        result := y;
+    }
+    gcd_correct(a,b);
+}
